
@prefix identity: <https://ontology.adversaryengagement.org/ae/identity/> . 
@prefix objective: <https://ontology.adversaryengagement.org/ae/objective/> . 
@prefix owl: <http://www.w3.org/2002/07/owl#> . 
@prefix rdfs: <http://www.w3.org/2000/01/rdf-schema#> . 
@prefix sh: <http://www.w3.org/ns/shacl#> . 
@prefix uco-core: <https://ontology.unifiedcyberontology.org/uco/core/> . 
@prefix xsd: <http://www.w3.org/2001/XMLSchema#> . 

 

objective:CommandAndControl a owl:Class, 
        sh:NodeShape ; 
    rdfs:label "CommandAndControl"@en ; 
    rdfs:comment " An CommandAndControl objective is defined by MITRE ATTACK tactic: Command and Control consists of techniques that adversaries may use to communicate with systems under their control within a victim network."@en ; 
    rdfs:subClassOf objective:Objective ;
    sh:targetClass objective:CommandAndControl . 
 

objective:CredentialAccess a owl:Class, 
        sh:NodeShape ; 
    rdfs:label "CredentialAccess"@en ; 
    rdfs:comment " An CredentialAccess objective is defined by MITRE ATTACK tactic: Credential Access consists of techniques for stealing credentials like account names and passwords."@en ; 
    rdfs:subClassOf objective:Objective ;
    sh:targetClass objective:CredentialAccess . 
 

objective:DevelopResource a owl:Class, 
        sh:NodeShape ; 
    rdfs:label "DevelopResource"@en ; 
    rdfs:comment " An DevelopResource (Resource Development) objective is defined by MITRE ATTACK tactic: Resource Development consists of techniques that involve adversaries creating, purchasing, or compromising/stealing resources that can be used to support targeting. Such resources include infrastructure, accounts, or capabilities."@en ; 
    rdfs:subClassOf objective:Objective ;
    sh:targetClass objective:DevelopResource . 
 

objective:Discover a owl:Class, 
        sh:NodeShape ; 
    rdfs:label "Discover"@en ; 
    rdfs:comment " An Discover (discovery) objective is defined by MITRE ATTACK tactic: Discovery consists of techniques an adversary may use to gain knowledge about the system and internal network."@en ; 
    rdfs:subClassOf objective:Objective ;
    sh:targetClass objective:Discover . 
 

objective:Evade a owl:Class, 
        sh:NodeShape ; 
    rdfs:label "Evade"@en ; 
    rdfs:comment " An evade objective is to avoid detection from some defense or entity."@en ; 
    rdfs:subClassOf objective:Objective ;
    sh:targetClass objective:Evade . 
 

objective:Execute a owl:Class, 
        sh:NodeShape ; 
    rdfs:label "Execute"@en ; 
    rdfs:comment " An Execute (Execution) objective is defined by MITRE ATTACK tactic: Execution consists of techniques that result in adversary-controlled code running on a local or remote system."@en ; 
    rdfs:subClassOf objective:Objective ;
    sh:targetClass objective:Execute . 
 

objective:Exfilitrate a owl:Class, 
        sh:NodeShape ; 
    rdfs:label "Exfilitrate"@en ; 
    rdfs:comment " An exfilitrate objective is an adversary objective to move native data to external sources."@en ; 
    rdfs:subClassOf objective:Objective ;
    sh:targetClass objective:Exfilitrate . 
 

objective:Impact a owl:Class, 
        sh:NodeShape ; 
    rdfs:label "Impact"@en ; 
    rdfs:comment " An Impact objective is defined by MITRE ATTACK tactic: Impact consists of techniques that adversaries use to disrupt availability or compromise integrity by manipulating business and operational processes."@en ; 
    rdfs:subClassOf objective:Objective ;
    sh:targetClass objective:Impact . 
 

objective:InitialAccess a owl:Class, 
        sh:NodeShape ; 
    rdfs:label "InitialAccess"@en ; 
    rdfs:comment " An InitialAccess objective is defined by MITRE ATTACK tactic: Initial Access consists of techniques that use various entry vectors to gain their initial foothold within a network."@en ; 
    rdfs:subClassOf objective:Objective ;
    sh:targetClass objective:InitialAccess . 
 

objective:LateralMove a owl:Class, 
        sh:NodeShape ; 
    rdfs:label "LateralMove"@en ; 
    rdfs:comment " An LateralMove(LateralMovement) objective is defined by MITRE ATTACK tactic: Lateral Movement consists of techniques that adversaries use to enter and control remote systems on a network."@en ; 
    rdfs:subClassOf objective:Objective ;
    sh:targetClass objective:LateralMove . 
 

objective:Persist a owl:Class, 
        sh:NodeShape ; 
    rdfs:label "Persist"@en ; 
    rdfs:comment " An persist objective is maintain availability and access to some resource."@en ; 
    rdfs:subClassOf objective:Objective ;
    sh:targetClass objective:Persist . 
 

objective:PrivilegeEscalate a owl:Class, 
        sh:NodeShape ; 
    rdfs:label "PrivilegeEscalate"@en ; 
    rdfs:comment " An PrivilegeEscalate(PrivilegeEscalation) objective is defined by MITRE ATTACK tactic: Privilege Escalation consists of techniques that adversaries use to gain higher-level permissions on a system or network."@en ; 
    rdfs:subClassOf objective:Objective ;
    sh:targetClass objective:PrivilegeEscalate . 
 

objective:Reconnaissance a owl:Class, 
        sh:NodeShape ; 
    rdfs:label "Reconnaissance"@en ; 
    rdfs:comment " An reconnaissance objective is to gather information on a target entity or organization including by not limited to behavior, tactics, techniques, procedures and preferences."@en ; 
    rdfs:subClassOf objective:Objective ;
    sh:targetClass objective:Reconnaissance . 
 

objective:Affect a owl:Class, 
        sh:NodeShape ; 
    rdfs:label "Affect"@en ; 
    rdfs:comment " An affect objective is defined by MITRE ENGAGE: Negatively impact the adversaries operations."@en ; 
    rdfs:subClassOf objective:Objective ;
    sh:targetClass objective:Affect . 
 

objective:Collect a owl:Class, 
        sh:NodeShape ; 
    rdfs:label "Collect"@en ; 
    rdfs:comment " A collect objective defined by MITRE ENGAGE: Gather adversary tools, observe tactics, and collect other raw intelligence about the adversary’s activity. Cocurrently, from MITRE ATTACK's Collection tactic: Collection consists of techniques adversaries may use to gather information and the sources information is collected from that are relevant to following through on the adversary's objectives."@en ; 
    rdfs:subClassOf objective:Objective ;
    sh:targetClass objective:Collect . 
 

objective:Detect a owl:Class, 
        sh:NodeShape ; 
    rdfs:label "Detect"@en ; 
    rdfs:comment " A detect objective defined by MITRE ENGAGE: Establish or maintain awareness regarding adversary activity."@en ; 
    rdfs:subClassOf objective:Objective ;
    sh:targetClass objective:Detect . 
 

objective:Direct a owl:Class, 
        sh:NodeShape ; 
    rdfs:label "Direct"@en ; 
    rdfs:comment " A direct objective defined by MITRE ENGAGE: Encourage or discourage the adversary from conducting their operation as intended. "@en ; 
    rdfs:subClassOf objective:Objective ;
    sh:targetClass objective:Direct . 
 

objective:Disrupt a owl:Class, 
        sh:NodeShape ; 
    rdfs:label "Disrupt"@en ; 
    rdfs:comment " A Disrupt objective defined by MITRE ENGAGE: Impair an adversary’s ability to conduct their operation as intended. "@en ; 
    rdfs:subClassOf objective:Objective ;
    sh:targetClass objective:Disrupt . 
 

objective:Elicit a owl:Class, 
        sh:NodeShape ; 
    rdfs:label "Elicit"@en ; 
    rdfs:comment " An affect objective is defined by MITRE ENGAGE: Learn about adversaries tactics, techniques, and procedures (TTPs)."@en ; 
    rdfs:subClassOf objective:Objective ;
    sh:targetClass objective:Elicit . 
 

objective:Expose a owl:Class, 
        sh:NodeShape ; 
    rdfs:label "Expose"@en ; 
    rdfs:comment " An expose objective is defined by MITRE ENGAGE: Reveal the presence of ongoing adversary operations."@en ; 
    rdfs:subClassOf objective:Objective ;
    sh:targetClass objective:Expose . 
 

objective:Motivate a owl:Class, 
        sh:NodeShape ; 
    rdfs:label "Motivate"@en ; 
    rdfs:comment " A Motivate objective defined by MITRE ENGAGE: Encourage an adversary to conduct part or all of their mission. "@en ; 
    rdfs:subClassOf objective:Objective ;
    sh:targetClass objective:Motivate . 
 

objective:Prevent a owl:Class, 
        sh:NodeShape ; 
    rdfs:label "Prevent"@en ; 
    rdfs:comment " A prevent objective defined by MITRE ENGAGE: Stop all or part of the adversary’s ability to conduct their operation as intended."@en ; 
    rdfs:subClassOf objective:Objective ;
    sh:targetClass objective:Prevent . 
 

objective:Reassure a owl:Class, 
        sh:NodeShape ; 
    rdfs:label "Reassure"@en ; 
    rdfs:comment " A Reassure objective defined by MITRE ENGAGE: Add authenticity to deceptive components to convince an adversary that an environment is real. "@en ; 
    rdfs:subClassOf objective:Objective ;
    sh:targetClass objective:Reassure . 
 

objective:Deny a owl:Class, 
        sh:NodeShape ; 
    rdfs:label "Denial"@en ; 
    rdfs:comment " An deny objective is to limit an adversary's capabilities or accessibility to a resource."@en ; 
    rdfs:subClassOf objective:Objective ;
    sh:targetClass objective:Deny . 
 

objective:ElicitBehavior a owl:Class, 
        sh:NodeShape ; 
    rdfs:label "ElicitBehavior"@en ; 
    rdfs:comment " An elicit behavior objective is to have an adversary or target object to exhibit some expected behavior."@en ; 
    rdfs:subClassOf objective:Objective ;
    sh:targetClass objective:ElicitBehavior . 
 

objective:hasObjective a owl:ObjectProperty, 
        sh:NodeShape ; 
    rdfs:label "hasObjective"@en ; 
    rdfs:comment "An object which can be associated with an objective."@en ; 
    rdfs:range uco-core:UcoObject .
 

objective:Lure a owl:Class, 
        sh:NodeShape ; 
    rdfs:label "Lure"@en ; 
    rdfs:comment " An lure objective is have an adversary laterally move or take actions to reach some target lure, usually performed through the deployment of breadcrumbs and honeypots."@en ; 
    rdfs:subClassOf objective:ElicitBehavior ;
    sh:targetClass objective:Lure . 


objective:Objective a owl:Class, 
        sh:NodeShape ; 
    rdfs:label "Objective"@en ; 
    rdfs:comment " An objective is a goal or goal-state associated with an object which is optimized for or desired to be satisified."@en ; 
    rdfs:subClassOf uco-core:UcoObject ;	
    sh:targetClass objective:Objective . 
 

objective:TimeSink a owl:Class, 
        sh:NodeShape ; 
    rdfs:label "TimeSink"@en ; 
    rdfs:comment " An time sink objective is to increase an adversary's operation time cost by having them interact with objects in a network."@en ; 
    rdfs:subClassOf objective:Objective ;
    sh:targetClass objective:TimeSink . 
 

objective:Track a owl:Class, 
        sh:NodeShape ; 
    rdfs:label "Track"@en ; 
    rdfs:comment " An track objective is to be capable of identifying and tracing an adversary throughout a network."@en ; 
    rdfs:subClassOf objective:Objective ;
    sh:targetClass objective:Track . 
 

objective:Trap a owl:Class, 
        sh:NodeShape ; 
    rdfs:label "Trap"@en ; 
    rdfs:comment " An trap objective is to limit an adversary's scope of reachability to a confined environment."@en ; 
    rdfs:subClassOf objective:Objective ,
		objective:Denial ;
    sh:targetClass objective:Trap . 