
@prefix attack: <https://ontology.adversaryengagement.org/ae/attack/> .
@prefix engage: <https://ontology.adversaryengagement.org/ae/engage/> . 
@prefix objective: <https://ontology.adversaryengagement.org/ae/objective/> . 
@prefix owl: <http://www.w3.org/2002/07/owl#> . 
@prefix pattern: <https://ontology.unifiedcyberontology.org/uco/pattern/> .
@prefix rdf: <http://www.w3.org/1999/02/22-rdf-syntax-ns#> . 
@prefix rdfs: <http://www.w3.org/2000/01/rdf-schema#> . 
@prefix role: <https://ontology.adversaryengagement.org/ae/role/> . 
@prefix sh: <http://www.w3.org/ns/shacl#> . 
@prefix time: <https://ontology.adversaryengagement.org/ae/time/> . 
@prefix uco-action: <https://ontology.unifiedcyberontology.org/uco/action/> .
@prefix uco-core: <https://ontology.unifiedcyberontology.org/uco/core/> . 
@prefix uco-identity: <https://ontology.unifiedcyberontology.org/uco/identity/> .
@prefix uco-observable: <https://ontology.unifiedcyberontology.org/uco/observable/> . 
@prefix uco-tool: <https://ontology.unifiedcyberontology.org/uco/tool/> . 
@prefix uco-vocabulary: <https://ontology.unifiedcyberontology.org/uco/vocabulary/> . 
@prefix vocabulary: <https://ontology.adversaryengagement.org/ae/vocabulary/> . 
@prefix xsd: <http://www.w3.org/2001/XMLSchema#> . 


 

engage:alert a owl:Class, 
        sh:NodeShape ; 
    rdfs:label "alert"@en ; 
    rdfs:comment " An alert is a notification or message generated by a monitoring tool or data source."@en ; 
    rdfs:subClassOf uco-core:UcoObject ; 
    sh:targetClass engage:alert . 
 

engage:breadcrumb a owl:Class, 
        sh:NodeShape ; 
    rdfs:label "breadcrumb"@en ; 
    rdfs:comment " A breadcrumb is a set of objects placed to be at least partially, sequentially interacted by an adversary to ellicit an explicit response, often in the context of lateral movement."@en ; 
    rdfs:subClassOf engage:Lure ; 
    sh:targetClass engage:breadcrumb . 


 
engage:breadcrumbFacet a owl:Class, 
        sh:NodeShape ; 
    rdfs:label "breadcrumbFacet"@en ; 
    rdfs:comment "A breadcrumb facet is a grouping of objects which are used to lure an adversary to a target resource."@en ; 
    rdfs:subClassOf uco-core:Facet ; 
    sh:property [ sh:class uco-observable:UcoObject ; 
            sh:maxCount 1 ; 
            sh:nodeKind sh:BlankNodeOrIRI ; 
            sh:path engage:deployEntity ], 
		[ sh:class uco-observable:UcoObject ; 
					sh:minCount 1 ; 
					sh:nodeKind sh:BlankNodeOrIRI ; 
					sh:path uco-observable:UcoObject ], 
		[ sh:class uco-observable:UcoObject ; 
					sh:nodeKind sh:BlankNodeOrIRI ; 
					sh:path engage:hasResource ] ;
    sh:targetClass engage:breadcrumbFacet . 
 

engage:convertsInto a owl:ObjectProperty ;
    rdfs:label "convertsInto"@en ; 
    rdfs:comment " ConvertsInto describe the relationship of two uco objects which are related through some transformation or resource allocation to support one continuous perception."@en ; 
    rdfs:range uco-core:UcoObject .

 

engage:dataSource a owl:Class, 
        sh:NodeShape ; 
    rdfs:label "dataSource"@en ; 
    rdfs:comment "a data source is some source that generates event logs which can be analyzed for adversary detection."@en ; 
    rdfs:subClassOf uco-core:UcoObject ; 
    sh:targetClass engage:dataSource . 
 

engage:deceptionTool a owl:Class, 
        sh:NodeShape ; 
    rdfs:label "deceptionTool"@en ; 
    rdfs:comment " A deception tool is a tool explicitly for adversary engagaement."@en ; 
    rdfs:subClassOf uco-tool:Tool ; 
    sh:targetClass engage:deceptionTool . 
 

engage:Decoy a owl:Class, 
        sh:NodeShape ; 
    rdfs:label "Lure"@en ; 
    rdfs:comment " A decoy is a placed object that has the perception of enough value to an adversary to pursue but contains no real value."@en ; 
    rdfs:subClassOf engage:LureObject ; 
    sh:targetClass engage:Decoy . 


engage:Deploy a owl:Class,
        sh:NodeShape ;
    rdfs:label "Deploy"@en ;
    rdfs:comment "Deploy is an action which some entity takes to instantiate some deception objects prior or during an operation."@en ;
    rdfs:subClassOf uco-action:Action ; 
	sh:property [ sh:datatype uco-core:UcoObject;
			sh:minCount 1 ;
			sh:nodeKind sh:Literal ;
			sh:path uco-identity:Identity ],
	[ sh:datatype uco-core:UcoObject ; 
		sh:minCount 1 ; 
		sh:nodeKind sh:Literal ; 
		sh:path engage:honeyObject ] ;
    sh:targetClass engage:Deploy .


engage:deployEntity a owl:ObjectProperty ;
    rdfs:label "deployEntity"@en ;
    rdfs:comment "Deploy entity is an entity that instantiates/configures some deception objects prior or during an operation."@en ;
    rdfs:range uco-core:Identity .


 
engage:DeployFacet a owl:Class, 
        sh:NodeShape ; 
    rdfs:label "DeployFacet"@en ; 
    rdfs:comment "A deploy facet is a grouping of entities that perform this action."@en ; 
    rdfs:subClassOf uco-core:Facet ; 
    sh:property [ sh:class uco-observable:UcoObject ; 
            sh:minCount 1 ; 
            sh:nodeKind sh:BlankNodeOrIRI ; 
            sh:path uco-identity:Identity ],
		[ sh:class uco-observable:UcoObject ; 
            sh:nodeKind sh:BlankNodeOrIRI ; 
            sh:path role:hasTeam ] ;
    sh:targetClass engage:honeyObjectFacet . 


engage:detect a owl:Class,
        sh:NodeShape ;
    rdfs:label "detect"@en ;
    rdfs:comment "Detect is an observational action which some entity identifies an adversarial entity, adversarial behaviors or signatures from data-source(s)."@en ;
    rdfs:subClassOf uco-action:Action ; 
    sh:targetClass engage:detect .
 
 

engage:Event a owl:Class, 
        sh:NodeShape ; 
    rdfs:label "Event"@en ; 
    rdfs:comment "An event is a collection of actions, entities, interactions designated to be performed at some sequentially indexed time in a narrative"@en ; 
    rdfs:subClassOf engage:Narrative ; 
    sh:targetClass engage:Event . 


 
engage:EventFacet a owl:Class, 
        sh:NodeShape ; 
    rdfs:label "EventFacet"@en ; 
    rdfs:comment "An event facet describes an event as a (entity, action, object/entity)."@en ; 
    rdfs:subClassOf uco-core:Facet ; 
    sh:property [ sh:class uco-observable:UcoObject ; 
            sh:nodeKind sh:BlankNodeOrIRI ; 
            sh:path uco-identity:Identity ],
		[ sh:class uco-observable:UcoObject ; 
            sh:nodeKind sh:BlankNodeOrIRI ; 
            sh:path uco-action:Action ],
		[ sh:class uco-observable:UcoObject ; 
            sh:nodeKind sh:BlankNodeOrIRI ; 
            sh:path uco-observable:UcoObject ] ;
    sh:targetClass engage:EventFacet . 




engage:Exit a owl:Class,
        sh:NodeShape ;
    rdfs:label "stagedAttackMethod"@en ;
    rdfs:comment "The exhibited method that allowed an actor to leave a specific stage."@en ;
    rdfs:subClassOf uco-core:UcoObject ;
    sh:targetClass attack:Exit .

 

engage:hasDataSource a owl:ObjectProperty, 
        sh:NodeShape ; 
    rdfs:label "hasDataSource"@en ; 
    rdfs:comment "a data source is some source that generates event logs which can be analyzed for adversary detection."@en ; 
    rdfs:range engage:dataSource .
 
 

engage:hasEvent a owl:ObjectProperty ;
    rdfs:label "hasEvent"@en ; 
    rdfs:comment "An object that can have an event object as a property."@en ; 
    rdfs:range engage:Event .

 

engage:hasHoneyObject a owl:ObjectProperty ;
    rdfs:label "hasHoneyObject"@en ; 
    rdfs:comment " An object that contains or is assigned additional honey objects."@en ; 
    rdfs:range engage:HoneyObject .

 

engage:hasResource a owl:ObjectProperty, 
        sh:NodeShape ; 
    rdfs:label "hasResource"@en ; 
    rdfs:comment "An object or entity that is associated with a resource."@en ; 
    rdfs:range engage:Resource .




engage:hasStage a owl:ObjectProperty ;
    rdfs:label "hasStage"@en ;
    rdfs:comment "A object that can be assigned or percieve to have a stage."@en ;
    rdfs:range engage:stage .




engage:hasStagedAttackMethod a owl:ObjectProperty ;
    rdfs:label "hasStagedAttackMethod"@en ;
    rdfs:comment "An expectation that an entity will use a specific attack methodology."@en ;
    rdfs:range engage:stagedAttackMethod .



engage:hasStagedExit a owl:ObjectProperty ;
    rdfs:label "hasStagedExit"@en ;
    rdfs:comment "An intended method of leaving a specific stage."@en ;
    rdfs:range engage:stagedExit .
 

engage:hasTool a owl:ObjectProperty ;
    rdfs:label "hasTool"@en ; 
    rdfs:comment " An object which uses or depends on a tool, software, or process."@en ; 
    rdfs:range uco-core:Tool .

 

engage:HoneyObject a owl:Class, 
        sh:NodeShape ; 
    rdfs:label "HoneyObject"@en ; 
    rdfs:comment " An domain object that is created to be percieved by an adversary to have high value to pursue in an adversary engagement operation."@en ; 
    rdfs:subClassOf engage:LureObject ; 
    sh:targetClass engage:HoneyObject . 


 
engage:HoneyObjectFacet a owl:Class, 
        sh:NodeShape ; 
    rdfs:label "HoneyObjectFacet"@en ; 
    rdfs:comment "A honey object facet is a grouping of characteristics that describe a honeyObject."@en ; 
    rdfs:subClassOf uco-core:Facet ; 
    sh:property [ sh:class uco-observable:UcoObject ; 
            sh:maxCount 1 ; 
            sh:nodeKind sh:BlankNodeOrIRI ; 
            sh:path engage:deployEntity ],
		[ sh:class uco-observable:UcoObject ; 
            sh:maxCount 1 ; 
            sh:nodeKind sh:BlankNodeOrIRI ; 
            sh:path engage:hasEvent ] ;
    sh:targetClass engage:honeyObjectFacet . 

 

engage:honeypot a owl:Class, 
        sh:NodeShape ; 
    rdfs:label "Honeypot"@en ; 
    rdfs:comment " A controlled environment intended to be probed, compromised or attacked by adversaries or malware."@en ; 
    rdfs:subClassOf engage:Decoy ,
		engage:HoneyObject ;
    sh:targetClass engage:honeypot . 


 
engage:HoneypotFacet a owl:Class, 
        sh:NodeShape ; 
    rdfs:label "HoneypotFacet"@en ; 
    rdfs:comment "A honeypot facet is a grouping of characteristics that describe the intentions or usage of the object in relationship to the adversary or adversary engagement mission."@en ; 
    rdfs:subClassOf uco-core:Facet ; 
    sh:property [ sh:class uco-core:UcoObject ; 
            sh:maxCount 1 ; 
            sh:nodeKind sh:BlankNodeOrIRI ; 
            sh:path engage:deployEntity ], 
		[ sh:class uco-core:UcoObject ; 
					sh:nodeKind sh:BlankNodeOrIRI ; 
					sh:path engage:hasStagedExit ], 
		[ sh:class uco-core:UcoObject ; 
					sh:nodeKind sh:BlankNodeOrIRI ; 
					sh:path engage:hasStage ], 
		[ sh:class attack:Attack ; 
					sh:nodeKind sh:BlankNodeOrIRI ; 
					sh:path engage:hasStagedAttackMethod ], 
		[ sh:class uco-tool:Tool ; 
					sh:nodeKind sh:BlankNodeOrIRI ; 
					sh:path engage:hasTool ], 
		[ sh:class engage:HoneyObject ; 
					sh:nodeKind sh:BlankNodeOrIRI ; 
					sh:path engage:hasHoneyObject ], 
		[ sh:class uco-core:UcoObject ; 
					sh:nodeKind sh:BlankNodeOrIRI ; 
					sh:path engage:convertsInto ], 
        [ sh:datatype xsd:dateTime ; 
            sh:maxCount 1 ; 
            sh:nodeKind sh:Literal ; 
            sh:path uco-observable:observableCreatedTime ], 
        [ sh:datatype xsd:dateTime ; 
            sh:maxCount 1 ; 
            sh:nodeKind sh:Literal ; 
            sh:path time:hasTime ], 
        [ sh:datatype vocabulary:HoneypotInteractionTypeVocab ; 
            sh:message "Value is outside the default vocabulary HoneypotInteractionTypeVocab." ; 
            sh:path engage:honeypotInteractionType ; 
            sh:severity sh:Info ], 
        [ sh:maxCount 1 ; 
            sh:nodeKind sh:Literal ; 
            sh:or ( [ sh:datatype vocabulary:HoneypotInteractionTypeVocab ] [ sh:datatype xsd:string ] ) ; 
            sh:path engage:honeypotInteractionType ], 
        [ sh:message "Value is not member of the vocabulary HoneypotInteractionTypeVocab." ; 
            sh:or ( [ sh:datatype vocabulary:HoneypotInteractionTypeVocab ; 
                        sh:in vocabulary:HoneypotInteractionTypeVocab-members ] [ sh:datatype xsd:string ] ) ; 
            sh:path engage:honeypotInteractionType ] ; 
    sh:targetClass engage:honeypotFacet . 

engage:honeypotInteractionType a owl:DatatypeProperty ;
    rdfs:label "honeypotInteractionType"@en ;
    rdfs:comment "The interaction class intended for a honeypot."@en ;
    rdfs:range [ a rdfs:Datatype ;
            owl:unionOf ( vocabulary:HoneypotInteractionTypeVocab xsd:string ) ] .

 

engage:honeyToken a owl:Class, 
        sh:NodeShape ; 
    rdfs:label "honeyToken"@en ; 
    rdfs:comment "A honey token gives an adversary direct access to a honeypot."@en ; 
    rdfs:subClassOf uco-core:UcoObject,
		engage:HoneyObject ;
    sh:targetClass engage:honeyToken . 


 
engage:honeyTokenFacet a owl:Class, 
        sh:NodeShape ; 
    rdfs:label "honeyTokenFacet"@en ; 
    rdfs:comment "A honey token facet is a grouping of characteristics for a honey token."@en ; 
    rdfs:subClassOf uco-core:Facet ; 
    sh:property [ sh:class uco-observable:UcoObject ; 
            sh:maxCount 1 ; 
            sh:nodeKind sh:BlankNodeOrIRI ; 
            sh:path engage:deployEntity ], 
		[ sh:class uco-observable:UcoObject ; 
					sh:nodeKind sh:BlankNodeOrIRI ; 
					sh:path uco-observable:Credential ] ; 
    sh:targetClass engage:honeyTokenFacet . 

 

engage:LureObject a owl:Class, 
        sh:NodeShape ; 
    rdfs:label "LureObject"@en ; 
    rdfs:comment " An object or set of objects used to attract an adversary."@en ; 
    rdfs:subClassOf uco-observable:ObservableObject ; 
    sh:targetClass engage:LureObject . 
 

engage:Malware a owl:Class, 
        sh:NodeShape ; 
    rdfs:label "Malware"@en ; 
    rdfs:comment "Malware is an explicit, complex, multi-functional, crafted tool, software, or program for malicious purposes. Not all malicious tools are Malware though."@en ; 
    rdfs:subClassOf uco-tool:MaliciousTool ; 
    sh:targetClass engage:Malware . 
 

engage:MalwareFacet a owl:Class, 
        sh:NodeShape ; 
    rdfs:label "MalwareFacet"@en ; 
    rdfs:comment "Malware facet is a collection of characteristics of Malware."@en ; 
    rdfs:subClassOf uco-core:Facet ; 
    sh:property [ sh:class uco-core:UcoObject ; 
            sh:maxCount 1 ; 
            sh:nodeKind sh:BlankNodeOrIRI ; 
            sh:path time:Time ] ,
	[ sh:class uco-core:UcoObject ; 
				sh:maxCount 1 ; 
				sh:nodeKind sh:BlankNodeOrIRI ; 
				sh:path engage:Deploy ];
    sh:targetClass engage:MalwareFacet . 

 

engage:Narrative a owl:Class, 
        sh:NodeShape ; 
    rdfs:label "Narrative"@en ; 
    rdfs:comment "A narrative is a script of expected sequence of actions, events, entities and their interactions."@en ; 
    rdfs:subClassOf uco-core:UcoObject ; 
    sh:targetClass engage:Narrative . 


engage:obfuscate a owl:Class,
        sh:NodeShape ;
    rdfs:label "obfuscate"@en ;
    rdfs:comment "Obfuscate is a transformative action an entity or tool performs to some object to reduce available information associated with that object."@en ;
    rdfs:subClassOf uco-action:Action,
		engage:respond ;
    sh:targetClass engage:obfuscate .

 

engage:pocketLitter a owl:Class, 
        sh:NodeShape ; 
    rdfs:label "pocketLitter"@en ; 
    rdfs:comment "Pocket litter describes objects placed prior or during an adversary engagement operation for the purpose of realism."@en ; 
    rdfs:subClassOf uco-core:UcoObject ; 
    sh:targetClass engage:pocketLitter . 

 

engage:Resource a owl:Class, 
        sh:NodeShape ; 
    rdfs:label "Resource"@en ; 
    rdfs:comment " A resource can be a tool, location or object which requires some operational cost to enable availability."@en ; 
    rdfs:subClassOf uco-observable:ObservableObject ; 
    sh:targetClass engage:Resource . 


engage:respond a owl:Class,
        sh:NodeShape ;
    rdfs:label "respond"@en ;
    rdfs:comment "Respond is a reactive, defensive action to some adversarial detection or alert."@en ;
    rdfs:subClassOf uco-action:Action ;
    sh:targetClass engage:respond .

 

engage:sandbox a owl:Class, 
        sh:NodeShape ; 
    rdfs:label "Sandbox"@en ; 
    rdfs:comment " A controlled environment intended for malware detonation."@en ; 
    rdfs:subClassOf uco-observable:ObservableObject ; 
    sh:targetClass engage:sandbox . 


 
engage:sandboxFacet a owl:Class, 
        sh:NodeShape ; 
    rdfs:label "sandboxFacet"@en ; 
    rdfs:comment "A sandbox facet is a grouping of characteristics that describe the intentions or usage of a sandbox."@en ; 
    rdfs:subClassOf uco-core:Facet ; 
    sh:property [ sh:class uco-core:UcoObject ; 
            sh:maxCount 1 ; 
            sh:nodeKind sh:BlankNodeOrIRI ; 
            sh:path engage:deployEntity ], 
		[ sh:class uco-core:UcoObject ; 
					sh:nodeKind sh:BlankNodeOrIRI ; 
					sh:path engage:hasStage ], 
		[ sh:class uco-tool:Tool ; 
					sh:nodeKind sh:BlankNodeOrIRI ; 
					sh:path engage:hasTool ], 
		[ sh:class engage:objective ; 
					sh:nodeKind sh:BlankNodeOrIRI ; 
					sh:path engage:hasObjective ], 
        [ sh:datatype xsd:dateTime ; 
            sh:maxCount 1 ; 
            sh:nodeKind sh:Literal ; 
            sh:path uco-observable:observableCreatedTime ], 
        [ sh:datatype xsd:dateTime ; 
            sh:maxCount 1 ; 
            sh:nodeKind sh:Literal ; 
            sh:path time:hasTime ],
	[ sh:class uco-core:UcoObject ; 
	sh:nodeKind sh:BlankNodeOrIRI ; 
	sh:path engage:hasDataSource ] ;
    sh:targetClass engage:sandboxFacet . 




engage:stage a owl:Class,
        sh:NodeShape ;
    rdfs:label "stage"@en ;
    rdfs:comment "A stage is a desired perception of an object or environment which actors act/perform within or upon."@en ;
    rdfs:subClassOf uco-core:Facet ,
		engage:Narrative ;
    sh:property [ sh:class uco-core:UcoObject ; 
            sh:nodeKind sh:BlankNodeOrIRI ; 
            sh:path uco-core:object ] ;
    sh:targetClass engage:stage .




engage:stagedAttackMethod a owl:Class,
        sh:NodeShape ;
    rdfs:label "stagedAttackMethod"@en ;
    rdfs:comment "An expectation that an entity will use a specific attack methodology."@en ;
    rdfs:subClassOf uco-action:Attack ;
    sh:targetClass attack:stagedAttackMethod .




engage:stagedAttackSurface a owl:Class,
        sh:NodeShape ;
    rdfs:label "stagedAttackMethod"@en ;
    rdfs:comment "An intentionally configured attack surface that is paired with a stagedAttackMethod."@en ;
    rdfs:subClassOf uco-core:UcoObject ;
    sh:targetClass attack:stagedAttackSurface .



engage:stagedExit a owl:Class,
        sh:NodeShape ;
    rdfs:label "stagedExit"@en ;
    rdfs:comment "An intended method of leaving a specific stage."@en ;
    rdfs:subClassOf uco-core:UcoObject ;
    sh:targetClass attack:stagedExit .

 

engage:Storyline a owl:Class, 
        sh:NodeShape ; 
    rdfs:label "Storyline"@en ; 
    rdfs:comment "A storyline is an indexed sequence of monotonic events."@en ; 
    rdfs:subClassOf engage:Narrative ; 
    sh:targetClass engage:Storyline . 