
@prefix attack: <https://ontology.adversaryengagement.org/ae/attack/> .
@prefix engage: <https://ontology.adversaryengagement.org/ae/engage/> .
@prefix identity: <https://ontology.adversaryengagement.org/ae/identity/> .
@prefix objective: <https://ontology.adversaryengagement.org/ae/objective/> .
@prefix owl: <http://www.w3.org/2002/07/owl#> .
@prefix pattern: <https://ontology.unifiedcyberontology.org/uco/pattern/> .
@prefix rdf: <http://www.w3.org/1999/02/22-rdf-syntax-ns#> .
@prefix rdfs: <http://www.w3.org/2000/01/rdf-schema#> .
@prefix role: <https://ontology.adversaryengagement.org/ae/role/> .
@prefix sh: <http://www.w3.org/ns/shacl#> .
@prefix time: <https://ontology.adversaryengagement.org/ae/time/> . 
@prefix uco-action: <https://ontology.unifiedcyberontology.org/uco/action/> .
@prefix uco-core: <https://ontology.unifiedcyberontology.org/uco/core/> . 
@prefix uco-identity: <https://ontology.unifiedcyberontology.org/uco/identity/> .
@prefix uco-observable: <https://ontology.unifiedcyberontology.org/uco/observable/> . 
@prefix uco-role: <https://ontology.unifiedcyberontology.org/uco/role/> .
@prefix vocabulary: <https://ontology.adversaryengagement.org/ae/vocabulary/> . 
@prefix xsd: <http://www.w3.org/2001/XMLSchema#> .





attack:AttackPattern a owl:Class,
        sh:NodeShape ;
    rdfs:label "AttackPattern"@en ;
    rdfs:comment "An attack pattern is some adversarial classification for a set of sub-actions from an attack framework that is associated with some objective."@en ;
    rdfs:subClassOf uco-action:ActionPattern ;
    sh:property [ sh:class engage:Objective ; 
					sh:nodeKind sh:IRI ; 
					sh:path objective:hasObjective ] ;
    sh:targetClass attack:AttackPattern .



attack:cyberKillChain a owl:Class,
        sh:NodeShape ;
    rdfs:label "cyberKillChain"@en ;
    rdfs:comment "An cyber kill chain is a ordered sequence of actions or events describing a lifecycle from some framework."@en ;
    rdfs:subClassOf uco-action:ActionLifecycle ;
    sh:targetClass attack:cyberKillChain .




attack:DefensePattern a owl:Class,
        sh:NodeShape ;
    rdfs:label "AttackPattern"@en ;
    rdfs:comment "An defense pattern is some defensive classification for a set of sub-actions from a defense framework that is associated with some objective."@en ;
    rdfs:subClassOf uco-action:ActionPattern ;
    sh:property [ sh:class engage:Objective ; 
					sh:nodeKind sh:IRI ; 
					sh:path objective:hasObjective ] ;
    sh:targetClass attack:DefensePattern .



engage:Access a owl:Class, 
        sh:NodeShape ; 
    rdfs:label "Access"@en ; 
    rdfs:comment " Access as an action refers to an observed or deduced interaction between an entity and an object."@en ; 
    rdfs:subClassOf uco-action:Action ; 
	sh:property [
		sh:datatype xsd:string ;
		sh:hasValue "access" ;
		sh:maxCount "1"^^xsd:integer ;
		sh:minCount "1"^^xsd:integer ;
		sh:nodeKind sh:Literal ;
		sh:path uco-core:name ;
	] ;
    sh:targetClass engage:Access . 


engage:Alert a owl:Class, 
        sh:NodeShape ; 
    rdfs:label "Alert"@en ; 
    rdfs:comment " An alert action relates a monitoring tool or data source that follows a detect action to an entity."@en ; 
    rdfs:subClassOf uco-action:Action ; 
	sh:property [
		sh:datatype xsd:string ;
		sh:hasValue "alert" ;
		sh:maxCount "1"^^xsd:integer ;
		sh:minCount "1"^^xsd:integer ;
		sh:nodeKind sh:Literal ;
		sh:path uco-core:name ;
	] ;
    sh:targetClass engage:Alert . 


engage:Deploy a owl:Class,
        sh:NodeShape ;
    rdfs:label "Deploy"@en ;
    rdfs:comment "Deploy is an action which some entity takes to instantiate some deception objects prior or during an operation."@en ;
    rdfs:subClassOf uco-action:Action ; 
	sh:property [
		sh:datatype xsd:string ;
		sh:hasValue "deploy" ;
		sh:maxCount "1"^^xsd:integer ;
		sh:minCount "1"^^xsd:integer ;
		sh:nodeKind sh:Literal ;
		sh:path uco-core:name ;
	] ;
    sh:targetClass engage:Deploy .


engage:Obfuscate a owl:Class,
        sh:NodeShape ;
    rdfs:label "Obfuscate"@en ;
    rdfs:comment "Obfuscate is a transformative action an entity or tool performs to some object to reduce available information associated with that object."@en ;
    rdfs:subClassOf engage:Respond ;
	sh:property [
		sh:datatype xsd:string ;
		sh:hasValue "obfuscate" ;
		sh:maxCount "1"^^xsd:integer ;
		sh:minCount "1"^^xsd:integer ;
		sh:nodeKind sh:Literal ;
		sh:path uco-core:name ;
	] ;
    sh:targetClass engage:Obfuscate .



engage:Respond a owl:Class,
        sh:NodeShape ;
    rdfs:label "Respond"@en ;
    rdfs:comment "Respond is a reactive, defensive action to some adversarial detection or alert."@en ;
    rdfs:subClassOf uco-action:Action ;
	sh:property [
		sh:datatype xsd:string ;
		sh:hasValue "respond" ;
		sh:maxCount "1"^^xsd:integer ;
		sh:minCount "1"^^xsd:integer ;
		sh:nodeKind sh:Literal ;
		sh:path uco-core:name ;
	] ;
    sh:targetClass engage:Respond .
 

engage:Breadcrumb a owl:Class, 
        sh:NodeShape ; 
    rdfs:label "Breadcrumb"@en ; 
    rdfs:comment " A Breadcrumb is a set of objects placed to be at least partially, sequentially interacted by an adversary to ellicit an explicit response, often in the context of lateral movement."@en ; 
    rdfs:subClassOf engage:LureObject ;
    sh:targetClass engage:Breadcrumb . 

 

engage:DataSource a owl:Class, 
        sh:NodeShape ; 
    rdfs:label "DataSource"@en ; 
    rdfs:comment "A data source is some source that generates event logs which can be analyzed for adversary detection."@en ; 
    rdfs:subClassOf uco-core:UcoObject ; 
    sh:targetClass engage:DataSource . 
 

engage:Decoy a owl:Class, 
        sh:NodeShape ; 
    rdfs:label "Decoy"@en ; 
    rdfs:comment " A decoy is a placed object that has the perception of enough value to an adversary to pursue but contains no real value."@en ; 
    rdfs:subClassOf engage:LureObject ; 
    sh:targetClass engage:Decoy . 

 

engage:HoneyObject a owl:Class, 
        sh:NodeShape ; 
    rdfs:label "HoneyObject"@en ; 
    rdfs:comment " An domain object that is created to be percieved by an adversary to have high value to pursue in an adversary engagement operation that has no value out of scope of the operation's intended perception."@en ; 
    rdfs:subClassOf engage:LureObject ; 
    sh:targetClass engage:HoneyObject . 


engage:Honeypot a owl:Class, 
        sh:NodeShape ; 
    rdfs:label "Honeypot"@en ; 
    rdfs:comment " A controlled environment intended to be probed, compromised or attacked by adversaries or malware."@en ; 
    rdfs:subClassOf engage:Decoy ,
		engage:HoneyObject ;
	sh:property [ sh:datatype vocabulary:HoneypotInteractionTypeVocab ;
		sh:message "Value is outside the default vocabulary HoneypotInteractionTypeVocab." ;
		sh:path engage:honeypotInteractionType ;
		sh:severity sh:Info ;] ,
	[ sh:maxCount "1"^^xsd:integer ;
		sh:nodeKind sh:Literal ;
		sh:or ([ sh:datatype vocabulary:HoneypotInteractionTypeVocab ;] [ sh:datatype xsd:string ;]) ;
		sh:path engage:honeypotInteractionType ;] ,
	[ sh:message "Value is not member of the vocabulary HoneypotInteractionTypeVocab." ;
		sh:or ([ sh:datatype vocabulary:HoneypotInteractionTypeVocab ;
				sh:in (
					"High"^^vocabulary:HoneypotTypeVocab
					"Low"^^vocabulary:HoneypotTypeVocab
					"Dynamic"^^vocabulary:HoneypotTypeVocab
				) ;
				] [ sh:datatype xsd:string ;]) ;
		sh:path engage:honeypotInteractionType ;] ;
    sh:targetClass engage:Honeypot . 

 

engage:HoneyToken a owl:Class, 
        sh:NodeShape ; 
    rdfs:label "HoneyToken"@en ; 
    rdfs:comment "A honey token gives an adversary direct access to a honeypot."@en ; 
    rdfs:subClassOf engage:HoneyObject ;
    sh:targetClass engage:HoneyToken . 

 

engage:LureObject a owl:Class, 
        sh:NodeShape ; 
    rdfs:label "LureObject"@en ; 
    rdfs:comment " An object or set of objects used to attract an adversary that has the perception of high value regardless if it actually has high value."@en ; 
    rdfs:subClassOf uco-core:UcoObject ;
    sh:property [ sh:class uco-core:UcoObject ;
            sh:minCount 1 ;
            sh:nodeKind sh:IRI ;
            sh:path engage:hasCharacterization ] ;
    sh:targetClass engage:LureObject . 
 

engage:Malware a owl:Class, 
        sh:NodeShape ; 
    rdfs:label "Malware"@en ; 
    rdfs:comment "Malware is an explicit, complex, multi-functional, crafted tool, software, or program for malicious purposes. Not all malicious tools are Malware though."@en ; 
    rdfs:subClassOf uco-core:UcoObject ; 
    sh:targetClass engage:Malware . 

 

engage:Narrative a owl:Class, 
        sh:NodeShape ; 
    rdfs:label "Narrative"@en ; 
    rdfs:comment "A narrative is a script of all expected sequence of actions, events, entities and their interactions."@en ; 
    rdfs:subClassOf uco-core:UcoObject ; 
    sh:property [ sh:class uco-core:UcoObject ;
            sh:minCount 1 ;
            sh:nodeKind sh:IRI ;
            sh:path engage:hasStoryline ] ,
		[ sh:class uco-core:UcoObject ;
					sh:minCount 1 ;
					sh:nodeKind sh:IRI ;
					sh:path engage:hasObjective ] ;
    sh:targetClass engage:Narrative . 

 

engage:PlannedEvent a owl:Class, 
        sh:NodeShape ; 
    rdfs:label "PlannedEvent"@en ; 
    rdfs:comment "An PlannedEvent is a collection of actions, entities, interactions designated to be performed at some sequentially indexed time in a narrative"@en ; 
    rdfs:subClassOf uco-core:UcoObject ; 
    sh:property [ sh:class uco-core:UcoObject ;
            sh:minCount 1 ;
            sh:nodeKind sh:IRI ;
            sh:path engage:eventContext ] ,
	[ sh:class uco-core:UcoObject ;
				sh:minCount 1 ;
				sh:nodeKind sh:IRI ;
				sh:path engage:hasObjective ] ;
    sh:targetClass engage:PlannedEvent . 

 

engage:PocketLitter a owl:Class, 
        sh:NodeShape ; 
    rdfs:label "PocketLitter"@en ; 
    rdfs:comment "Pocket litter describes objects placed prior or during an adversary engagement operation for the purpose of realism."@en ; 
    rdfs:subClassOf uco-core:UcoObject ; 
    sh:property [ sh:class uco-core:UcoObject ;
            sh:minCount 1 ;
            sh:nodeKind sh:IRI ;
            sh:path engage:hasCharacterization ] ;
    sh:targetClass engage:PocketLitter . 

 

engage:Resource a owl:Class, 
        sh:NodeShape ; 
    rdfs:label "Resource"@en ; 
    rdfs:comment " A resource can be a tool, location or object which requires some operational cost to enable availability."@en ; 
    rdfs:subClassOf uco-core:UcoObject ; 
    sh:targetClass engage:Resource . 

 

engage:Sandbox a owl:Class, 
        sh:NodeShape ; 
    rdfs:label "Sandbox"@en ; 
    rdfs:comment " A controlled environment intended for malware detonation and malware analysis."@en ; 
    rdfs:subClassOf uco-core:UcoObject ; 
    sh:targetClass engage:Sandbox . 




engage:Stage a owl:Class,
        sh:NodeShape ;
    rdfs:label "Stage"@en ;
    rdfs:comment "A stage is a desired perception of an object or environment for an intended audience or entity which actors act/perform within and upon."@en ;
    rdfs:subClassOf uco-core:UcoObject ;
    sh:property [ sh:class uco-core:UcoObject ;
            sh:minCount 1 ;
            sh:nodeKind sh:IRI ;
            sh:path engage:hasCharacterization ] ;
    sh:targetClass engage:Stage .




engage:StageAttackSurface a owl:Class,
        sh:NodeShape ;
    rdfs:label "StageAttackSurface"@en ;
    rdfs:comment "An intentionally configured attack surface described by UcoObjects."@en ;
    rdfs:subClassOf uco-core:UcoObject ;
    sh:property [ sh:class uco-core:UcoObject ;
            sh:minCount 1 ;
            sh:nodeKind sh:IRI ;
            sh:path engage:hasCharacterization ] ;
    sh:targetClass engage:StageAttackSurface .

 

engage:Storyline a owl:Class, 
        sh:NodeShape ; 
    rdfs:label "Storyline"@en ; 
    rdfs:comment "A storyline is an indexed sequence of monotonic events as an expected trajectory for a narrative."@en ; 
    rdfs:subClassOf uco-core:UcoObject ; 
    sh:targetClass engage:Storyline . 
 

engage:alertContext a owl:ObjectProperty, 
        sh:NodeShape ; 
    rdfs:label "alertContext"@en ; 
    rdfs:comment "An alert context describes the association of actions and objects relating to an alert."@en ; 
    rdfs:range uco-core:UcoObject .
 

engage:eventContext a owl:ObjectProperty, 
        sh:NodeShape ; 
    rdfs:label "eventContext"@en ; 
    rdfs:comment "An event context describes the association of actions and objects relating to an event."@en ; 
    rdfs:range uco-core:UcoObject .
 

engage:hasCharacterization a owl:ObjectProperty, 
        sh:NodeShape ; 
    rdfs:label "hasCharacterization"@en ; 
    rdfs:comment "hasCharacterization is an object property which describes the literal UcoObjects which compose a deception object or adversary engagement concept."@en ; 
    rdfs:range uco-core:UcoObject .
 

engage:hasEvent a owl:ObjectProperty, 
        sh:NodeShape ; 
    rdfs:label "hasEvent"@en ; 
    rdfs:comment "hasEvent is the event property associated exclusively with an event."@en ; 
    rdfs:range engage:Event .
 

engage:hasStoryline a owl:ObjectProperty, 
        sh:NodeShape ; 
    rdfs:label "hasStoryline"@en ; 
    rdfs:comment "A storyline is exclusive to a narrative."@en ; 
    rdfs:range engage:Storyline .

engage:honeypotInteractionType a owl:DatatypeProperty ;
    rdfs:label "honeypotInteractionType"@en ;
    rdfs:comment "The interaction class intended for a honeypot."@en ;
    rdfs:range [ a rdfs:Datatype ;
            owl:unionOf ( vocabulary:HoneypotInteractionTypeVocab xsd:string ) ] .


 
	
objective:BlueTeam a identity:Team ;
  rdfs:label "BlueTeam"@en;
  rdfs:comment "An BlueTeam is an instance of a team with defender objectives."@en;
  rdfs:range	uco-identity:Organization .


 

engage:Persona a owl:Class, 
        sh:NodeShape ; 
    rdfs:label "Persona"@en ; 
    rdfs:comment " An persona is a facticious entity created to serve a purpose in a deception operation."@en ; 
    rdfs:subClassOf uco-identity:Identity ;
    sh:targetClass engage:Persona . 

 
	
objective:PurpleTeam a identity:Team ;
  rdfs:label "PurpleTeam"@en;
  rdfs:comment "An PurpleTeam is an instance of a team with post analysis objectives."@en;
  rdfs:range	uco-identity:Organization .


 
	
objective:RedTeam a identity:Team ;
  rdfs:label "RedTeam"@en;
  rdfs:comment "An RedTeam is an instance of a team with adversary objectives."@en;
  rdfs:range	uco-identity:Organization .



role:Team a owl:Class,
        sh:NodeShape ;
    rdfs:label "Team"@en ;
    rdfs:comment "The conventional reference to group of identities that are associated with some unified identity with a team objective"@en ;
    rdfs:subClassOf uco-identity:Organization ;
    sh:property [ sh:class engage:Objective ;
            sh:nodeKind sh:IRI ;
            sh:path objective:hasObjective ] ;
    sh:targetClass role:Team .
	


 

objective:CommandAndControl a owl:Class, 
        sh:NodeShape ; 
    rdfs:label "CommandAndControl"@en ; 
    rdfs:comment " An CommandAndControl objective is defined by MITRE ATTACK tactic: Command and Control consists of techniques that adversaries may use to communicate with systems under their control within a victim network."@en ; 
    rdfs:subClassOf objective:Objective ;
    sh:targetClass objective:CommandAndControl . 
 

objective:CredentialAccess a owl:Class, 
        sh:NodeShape ; 
    rdfs:label "CredentialAccess"@en ; 
    rdfs:comment " An CredentialAccess objective is defined by MITRE ATTACK tactic: Credential Access consists of techniques for stealing credentials like account names and passwords."@en ; 
    rdfs:subClassOf objective:Objective ;
    sh:targetClass objective:CredentialAccess . 
 

objective:DevelopResource a owl:Class, 
        sh:NodeShape ; 
    rdfs:label "DevelopResource"@en ; 
    rdfs:comment " An DevelopResource (Resource Development) objective is defined by MITRE ATTACK tactic: Resource Development consists of techniques that involve adversaries creating, purchasing, or compromising/stealing resources that can be used to support targeting. Such resources include infrastructure, accounts, or capabilities."@en ; 
    rdfs:subClassOf objective:Objective ;
    sh:targetClass objective:DevelopResource . 
 

objective:Discover a owl:Class, 
        sh:NodeShape ; 
    rdfs:label "Discover"@en ; 
    rdfs:comment " An Discover (discovery) objective is defined by MITRE ATTACK tactic: Discovery consists of techniques an adversary may use to gain knowledge about the system and internal network."@en ; 
    rdfs:subClassOf objective:Objective ;
    sh:targetClass objective:Discover . 
 

objective:Evade a owl:Class, 
        sh:NodeShape ; 
    rdfs:label "Evade"@en ; 
    rdfs:comment " An evade objective is to avoid detection from some defense or entity."@en ; 
    rdfs:subClassOf objective:Objective ;
    sh:targetClass objective:Evade . 
 

objective:Execute a owl:Class, 
        sh:NodeShape ; 
    rdfs:label "Execute"@en ; 
    rdfs:comment " An Execute (Execution) objective is defined by MITRE ATTACK tactic: Execution consists of techniques that result in adversary-controlled code running on a local or remote system."@en ; 
    rdfs:subClassOf objective:Objective ;
    sh:targetClass objective:Execute . 
 

objective:Exfilitrate a owl:Class, 
        sh:NodeShape ; 
    rdfs:label "Exfilitrate"@en ; 
    rdfs:comment " An exfilitrate objective is an adversary objective to move native data to external sources."@en ; 
    rdfs:subClassOf objective:Objective ;
    sh:targetClass objective:Exfilitrate . 
 

objective:Impact a owl:Class, 
        sh:NodeShape ; 
    rdfs:label "Impact"@en ; 
    rdfs:comment " An Impact objective is defined by MITRE ATTACK tactic: Impact consists of techniques that adversaries use to disrupt availability or compromise integrity by manipulating business and operational processes."@en ; 
    rdfs:subClassOf objective:Objective ;
    sh:targetClass objective:Impact . 
 

objective:InitialAccess a owl:Class, 
        sh:NodeShape ; 
    rdfs:label "InitialAccess"@en ; 
    rdfs:comment " An InitialAccess objective is defined by MITRE ATTACK tactic: Initial Access consists of techniques that use various entry vectors to gain their initial foothold within a network."@en ; 
    rdfs:subClassOf objective:Objective ;
    sh:targetClass objective:InitialAccess . 
 

objective:LateralMove a owl:Class, 
        sh:NodeShape ; 
    rdfs:label "LateralMove"@en ; 
    rdfs:comment " An LateralMove(LateralMovement) objective is defined by MITRE ATTACK tactic: Lateral Movement consists of techniques that adversaries use to enter and control remote systems on a network."@en ; 
    rdfs:subClassOf objective:Objective ;
    sh:targetClass objective:LateralMove . 
 

objective:Persist a owl:Class, 
        sh:NodeShape ; 
    rdfs:label "Persist"@en ; 
    rdfs:comment " An persist objective is maintain availability and access to some resource."@en ; 
    rdfs:subClassOf objective:Objective ;
    sh:targetClass objective:Persist . 
 

objective:PrivilegeEscalate a owl:Class, 
        sh:NodeShape ; 
    rdfs:label "PrivilegeEscalate"@en ; 
    rdfs:comment " An PrivilegeEscalate(PrivilegeEscalation) objective is defined by MITRE ATTACK tactic: Privilege Escalation consists of techniques that adversaries use to gain higher-level permissions on a system or network."@en ; 
    rdfs:subClassOf objective:Objective ;
    sh:targetClass objective:PrivilegeEscalate . 
 

objective:Reconnaissance a owl:Class, 
        sh:NodeShape ; 
    rdfs:label "Reconnaissance"@en ; 
    rdfs:comment " An reconnaissance objective is to gather information on a target entity or organization including by not limited to behavior, tactics, techniques, procedures and preferences."@en ; 
    rdfs:subClassOf objective:Objective ;
    sh:targetClass objective:Reconnaissance . 
 

objective:Affect a owl:Class, 
        sh:NodeShape ; 
    rdfs:label "Affect"@en ; 
    rdfs:comment " An affect objective is defined by MITRE ENGAGE: Negatively impact the adversaries operations."@en ; 
    rdfs:subClassOf objective:Objective ;
    sh:targetClass objective:Affect . 
 

objective:Collect a owl:Class, 
        sh:NodeShape ; 
    rdfs:label "Collect"@en ; 
    rdfs:comment " A collect objective defined by MITRE ENGAGE: Gather adversary tools, observe tactics, and collect other raw intelligence about the adversary’s activity. Cocurrently, from MITRE ATTACK's Collection tactic: Collection consists of techniques adversaries may use to gather information and the sources information is collected from that are relevant to following through on the adversary's objectives."@en ; 
    rdfs:subClassOf objective:Objective ;
    sh:targetClass objective:Collect . 
 

objective:Detect a owl:Class, 
        sh:NodeShape ; 
    rdfs:label "Detect"@en ; 
    rdfs:comment " A detect objective defined by MITRE ENGAGE: Establish or maintain awareness regarding adversary activity."@en ; 
    rdfs:subClassOf objective:Objective ;
    sh:targetClass objective:Detect . 
 

objective:Direct a owl:Class, 
        sh:NodeShape ; 
    rdfs:label "Direct"@en ; 
    rdfs:comment " A direct objective defined by MITRE ENGAGE: Encourage or discourage the adversary from conducting their operation as intended. "@en ; 
    rdfs:subClassOf objective:Objective ;
    sh:targetClass objective:Direct . 
 

objective:Disrupt a owl:Class, 
        sh:NodeShape ; 
    rdfs:label "Disrupt"@en ; 
    rdfs:comment " A Disrupt objective defined by MITRE ENGAGE: Impair an adversary’s ability to conduct their operation as intended. "@en ; 
    rdfs:subClassOf objective:Objective ;
    sh:targetClass objective:Disrupt . 
 

objective:Elicit a owl:Class, 
        sh:NodeShape ; 
    rdfs:label "Elicit"@en ; 
    rdfs:comment " An affect objective is defined by MITRE ENGAGE: Learn about adversaries tactics, techniques, and procedures (TTPs)."@en ; 
    rdfs:subClassOf objective:Objective ;
    sh:targetClass objective:Elicit . 
 

objective:Expose a owl:Class, 
        sh:NodeShape ; 
    rdfs:label "Expose"@en ; 
    rdfs:comment " An expose objective is defined by MITRE ENGAGE: Reveal the presence of ongoing adversary operations."@en ; 
    rdfs:subClassOf objective:Objective ;
    sh:targetClass objective:Expose . 
 

objective:Motivate a owl:Class, 
        sh:NodeShape ; 
    rdfs:label "Motivate"@en ; 
    rdfs:comment " A Motivate objective defined by MITRE ENGAGE: Encourage an adversary to conduct part or all of their mission. "@en ; 
    rdfs:subClassOf objective:Objective ;
    sh:targetClass objective:Motivate . 
 

objective:Prevent a owl:Class, 
        sh:NodeShape ; 
    rdfs:label "Prevent"@en ; 
    rdfs:comment " A prevent objective defined by MITRE ENGAGE: Stop all or part of the adversary’s ability to conduct their operation as intended."@en ; 
    rdfs:subClassOf objective:Objective ;
    sh:targetClass objective:Prevent . 
 

objective:Reassure a owl:Class, 
        sh:NodeShape ; 
    rdfs:label "Reassure"@en ; 
    rdfs:comment " A Reassure objective defined by MITRE ENGAGE: Add authenticity to deceptive components to convince an adversary that an environment is real. "@en ; 
    rdfs:subClassOf objective:Objective ;
    sh:targetClass objective:Reassure . 
 

objective:Deny a owl:Class, 
        sh:NodeShape ; 
    rdfs:label "Denial"@en ; 
    rdfs:comment " An deny objective is to limit an adversary's capabilities or accessibility to a resource."@en ; 
    rdfs:subClassOf objective:Objective ;
    sh:targetClass objective:Deny . 
 

objective:ElicitBehavior a owl:Class, 
        sh:NodeShape ; 
    rdfs:label "ElicitBehavior"@en ; 
    rdfs:comment " An elicit behavior objective is to have an adversary or target object to exhibit some expected behavior."@en ; 
    rdfs:subClassOf objective:Objective ;
    sh:targetClass objective:ElicitBehavior . 
 

objective:hasObjective a owl:ObjectProperty, 
        sh:NodeShape ; 
    rdfs:label "hasObjective"@en ; 
    rdfs:comment "An object which can be associated with an objective."@en ; 
    rdfs:range uco-core:UcoObject .
 

objective:Lure a owl:Class, 
        sh:NodeShape ; 
    rdfs:label "Lure"@en ; 
    rdfs:comment " An lure objective is have an adversary laterally move or take actions to reach some target lure, usually performed through the deployment of breadcrumbs and honeypots."@en ; 
    rdfs:subClassOf objective:ElicitBehavior ;
    sh:targetClass objective:Lure . 


objective:Objective a owl:Class, 
        sh:NodeShape ; 
    rdfs:label "Objective"@en ; 
    rdfs:comment " An objective is a goal or goal-state associated with an object which is optimized for or desired to be satisified."@en ; 
    rdfs:subClassOf uco-core:UcoObject ;	
    sh:targetClass objective:Objective . 
 

objective:TimeSink a owl:Class, 
        sh:NodeShape ; 
    rdfs:label "TimeSink"@en ; 
    rdfs:comment " An time sink objective is to increase an adversary's operation time cost by having them interact with objects in a network."@en ; 
    rdfs:subClassOf objective:Objective ;
    sh:targetClass objective:TimeSink . 
 

objective:Track a owl:Class, 
        sh:NodeShape ; 
    rdfs:label "Track"@en ; 
    rdfs:comment " An track objective is to be capable of identifying and tracing an adversary throughout a network."@en ; 
    rdfs:subClassOf objective:Objective ;
    sh:targetClass objective:Track . 
 

objective:Trap a owl:Class, 
        sh:NodeShape ; 
    rdfs:label "Trap"@en ; 
    rdfs:comment " An trap objective is to limit an adversary's scope of reachability to a confined environment."@en ; 
    rdfs:subClassOf objective:Objective ,
		objective:Denial ;
    sh:targetClass objective:Trap . 


 
	
objective:Adversary a uco-role:Role ;
  rdfs:label "Adversary"@en;
  rdfs:comment "An adversary is an instance of a contextualized role that holds opposing interests to a defender role."@en;
  rdfs:range	uco-identity:Identity .


 
	
objective:Defender a uco-role:Role ;
  rdfs:label "Defender"@en;
  rdfs:comment "An defender is an instance of a contextualized role that defends some object or asset for some objective."@en;
  rdfs:range	uco-identity:Identity .




vocabulary:HoneypotInteractionTypeVocab a rdfs:Datatype ;
    rdfs:label "Action Name Vocabulary"@en-US ;
    rdfs:comment "Defines a vocabulary of honeypot interaction characteristics."@en ;
    rdfs:subClassOf rdfs:Resource ;
    owl:oneOf ( "High"^^vocabulary:HoneypotTypeVocab "Low"^^vocabulary:HoneypotTypeVocab "Dynamic"^^vocabulary:HoneypotTypeVocab ) .

