
@prefix attack: <https://ontology.adversaryengagement.org/ae/attack/> .
@prefix engage: <https://ontology.adversaryengagement.org/ae/engage/> . 
@prefix identity: <https://ontology.adversaryengagement.org/ae/identity/> .
@prefix objective: <https://ontology.adversaryengagement.org/ae/objective/> .
@prefix owl: <http://www.w3.org/2002/07/owl#> .
@prefix pattern: <https://ontology.unifiedcyberontology.org/uco/pattern/> .
@prefix rdf: <http://www.w3.org/1999/02/22-rdf-syntax-ns#> .
@prefix rdfs: <http://www.w3.org/2000/01/rdf-schema#> .
@prefix role: <https://ontology.adversaryengagement.org/ae/role/> .
@prefix sh: <http://www.w3.org/ns/shacl#> .
@prefix time: <https://ontology.adversaryengagement.org/ae/time/> . 
@prefix uco-action: <https://ontology.unifiedcyberontology.org/uco/action/> .
@prefix uco-core: <https://ontology.unifiedcyberontology.org/uco/core/> . 
@prefix uco-identity: <https://ontology.unifiedcyberontology.org/uco/identity/> .
@prefix uco-observable: <https://ontology.unifiedcyberontology.org/uco/observable/> . 
@prefix uco-role: <https://ontology.unifiedcyberontology.org/uco/role/> .
@prefix uco-tool: <https://ontology.unifiedcyberontology.org/uco/tool/> . 
@prefix vocabulary: <https://ontology.adversaryengagement.org/ae/vocabulary/> . 
@prefix xsd: <http://www.w3.org/2001/XMLSchema#> .





attack:Attack a owl:Class,
        sh:NodeShape ;
    rdfs:label "Attack"@en ;
    rdfs:comment "An attack is some adversarial behavioral classification from an attack framework."@en ;
    rdfs:subClassOf attack:AttackPattern ;
    sh:targetClass attack:Attack .



attack:AttackPattern a owl:Class,
        sh:NodeShape ;
    rdfs:label "AttackPattern"@en ;
    rdfs:comment "An attack pattern is some adversarial classification for a set of sub-actions from an attack framework that is associated with some objective."@en ;
    rdfs:subClassOf uco-action:ActionPattern ;
    sh:property [ sh:datatype xsd:Literal ;
            sh:maxCount 1 ;
            sh:nodeKind sh:BlankNodeOrIRI ;
            sh:path identity:techniqueIdentifier ] ,
		[ sh:datatype xsd:Literal ;
				sh:maxCount 1 ;
				sh:nodeKind sh:BlankNodeOrIRI ;
				sh:path identity:tacticIdentifier ] ,
		[ sh:class engage:Objective ; 
					sh:nodeKind sh:BlankNodeOrIRI ; 
					sh:path objective:hasObjective ] ;
    sh:targetClass attack:AttackPattern .



attack:cyberKillChain a owl:Class,
        sh:NodeShape ;
    rdfs:label "cyberKillChain"@en ;
    rdfs:comment "An cyber kill chain is a ordered sequence of actions or events describing a lifecycle from some framework."@en ;
    rdfs:subClassOf uco-action:ActionLifecycle ;
    sh:targetClass attack:cyberKillChain .



engage:Access a owl:Class, 
        sh:NodeShape ; 
    rdfs:label "Access"@en ; 
    rdfs:comment " Access as an action refers to an observed or deduced interaction between an entity and an object."@en ; 
    rdfs:subClassOf uco-action:Action ; 
	sh:property [
		sh:datatype xsd:string ;
		sh:hasValue "access" ;
		sh:maxCount "1"^^xsd:integer ;
		sh:minCount "1"^^xsd:integer ;
		sh:nodeKind sh:Literal ;
		sh:path uco-core:name ;
	] ;
    sh:targetClass engage:Access . 


engage:Alert a owl:Class, 
        sh:NodeShape ; 
    rdfs:label "Alert"@en ; 
    rdfs:comment " An alert action relates a monitoring tool or data source that follows a detect action to an entity."@en ; 
    rdfs:subClassOf uco-action:Action ; 
	sh:property [
		sh:datatype xsd:string ;
		sh:hasValue "alert" ;
		sh:maxCount "1"^^xsd:integer ;
		sh:minCount "1"^^xsd:integer ;
		sh:nodeKind sh:Literal ;
		sh:path uco-core:name ;
	] ;
    sh:targetClass engage:Alert . 


engage:Deploy a owl:Class,
        sh:NodeShape ;
    rdfs:label "Deploy"@en ;
    rdfs:comment "Deploy is an action which some entity takes to instantiate some deception objects prior or during an operation."@en ;
    rdfs:subClassOf uco-action:Action ; 
	sh:property [
		sh:datatype xsd:string ;
		sh:hasValue "deploy" ;
		sh:maxCount "1"^^xsd:integer ;
		sh:minCount "1"^^xsd:integer ;
		sh:nodeKind sh:Literal ;
		sh:path uco-core:name ;
	] ;
    sh:targetClass engage:Deploy .



engage:Detect a owl:Class,
        sh:NodeShape ;
    rdfs:label "Detect"@en ;
    rdfs:comment "Detect is an observational action which some entity identifies an adversarial entity, adversarial behaviors or signatures from data-source(s)."@en ;
    rdfs:subClassOf uco-action:Action ; 
	sh:property [
		sh:datatype xsd:string ;
		sh:hasValue "detect" ;
		sh:maxCount "1"^^xsd:integer ;
		sh:minCount "1"^^xsd:integer ;
		sh:nodeKind sh:Literal ;
		sh:path uco-core:name ;
	] ;
    sh:targetClass engage:Detect .


engage:Obfuscate a owl:Class,
        sh:NodeShape ;
    rdfs:label "Obfuscate"@en ;
    rdfs:comment "Obfuscate is a transformative action an entity or tool performs to some object to reduce available information associated with that object."@en ;
    rdfs:subClassOf uco-action:Action,
		engage:respond ;
	sh:property [
		sh:datatype xsd:string ;
		sh:hasValue "obfuscate" ;
		sh:maxCount "1"^^xsd:integer ;
		sh:minCount "1"^^xsd:integer ;
		sh:nodeKind sh:Literal ;
		sh:path uco-core:name ;
	] ;
    sh:targetClass engage:Obfuscate .



engage:Respond a owl:Class,
        sh:NodeShape ;
    rdfs:label "Respond"@en ;
    rdfs:comment "Respond is a reactive, defensive action to some adversarial detection or alert."@en ;
    rdfs:subClassOf uco-action:Action ;
	sh:property [
		sh:datatype xsd:string ;
		sh:hasValue "respond" ;
		sh:maxCount "1"^^xsd:integer ;
		sh:minCount "1"^^xsd:integer ;
		sh:nodeKind sh:Literal ;
		sh:path uco-core:name ;
	] ;
    sh:targetClass engage:Respond .
 

engage:Breadcrumb a owl:Class, 
        sh:NodeShape ; 
    rdfs:label "Breadcrumb"@en ; 
    rdfs:comment " A Breadcrumb is a set of objects placed to be at least partially, sequentially interacted by an adversary to ellicit an explicit response, often in the context of lateral movement."@en ; 
    rdfs:subClassOf engage:LureObject ; 
    sh:targetClass engage:Breadcrumb . 

 

engage:DataSource a owl:Class, 
        sh:NodeShape ; 
    rdfs:label "DataSource"@en ; 
    rdfs:comment "A data source is some source that generates event logs which can be analyzed for adversary detection."@en ; 
    rdfs:subClassOf uco-core:UcoObject ; 
    sh:targetClass engage:DataSource . 
 

engage:Decoy a owl:Class, 
        sh:NodeShape ; 
    rdfs:label "Decoy"@en ; 
    rdfs:comment " A decoy is a placed object that has the perception of enough value to an adversary to pursue but contains no real value."@en ; 
    rdfs:subClassOf engage:LureObject ; 
    sh:targetClass engage:Decoy . 

 

engage:Event a owl:Class, 
        sh:NodeShape ; 
    rdfs:label "Event"@en ; 
    rdfs:comment "An event is a collection of actions, entities, interactions designated to be performed at some sequentially indexed time in a narrative"@en ; 
    rdfs:subClassOf uco-core:UcoObject ; 
    sh:property [ sh:class uco-core:UcoObject ;
            sh:minCount 1 ;
            sh:nodeKind sh:BlankNodeOrIRI ;
            sh:path engage:hasEventScript ] ;
    sh:targetClass engage:Event . 

 

engage:HoneyObject a owl:Class, 
        sh:NodeShape ; 
    rdfs:label "HoneyObject"@en ; 
    rdfs:comment " An domain object that is created to be percieved by an adversary to have high value to pursue in an adversary engagement operation that has no value out of scope of the operation's intended perception."@en ; 
    rdfs:subClassOf engage:LureObject ; 
    sh:targetClass engage:HoneyObject . 


engage:Honeypot a owl:Class, 
        sh:NodeShape ; 
    rdfs:label "Honeypot"@en ; 
    rdfs:comment " A controlled environment intended to be probed, compromised or attacked by adversaries or malware."@en ; 
    rdfs:subClassOf engage:Decoy ,
		engage:HoneyObject ;
    sh:property [ sh:datatype vocabulary:HoneypotInteractionTypeVocab ; 
            sh:message "Value is outside the default vocabulary HoneypotInteractionTypeVocab." ; 
            sh:path engage:honeypotInteractionType ; 
            sh:severity sh:Info ], 
        [ sh:maxCount 1 ; 
            sh:nodeKind sh:Literal ; 
            sh:or ( [ sh:datatype vocabulary:HoneypotInteractionTypeVocab ] [ sh:datatype xsd:string ] ) ; 
            sh:path engage:honeypotInteractionType ], 
        [ sh:message "Value is not member of the vocabulary HoneypotInteractionTypeVocab." ; 
            sh:or ( [ sh:datatype vocabulary:HoneypotInteractionTypeVocab ; 
                        sh:in vocabulary:HoneypotInteractionTypeVocab-members ] [ sh:datatype xsd:string ] ) ; 
            sh:path engage:honeypotInteractionType ] ; 
    sh:targetClass engage:Honeypot . 

 

engage:HoneyToken a owl:Class, 
        sh:NodeShape ; 
    rdfs:label "HoneyToken"@en ; 
    rdfs:comment "A honey token gives an adversary direct access to a honeypot."@en ; 
    rdfs:subClassOf uco-core:UcoObject,
		engage:HoneyObject ;
    sh:targetClass engage:HoneyToken . 

 

engage:LureObject a owl:Class, 
        sh:NodeShape ; 
    rdfs:label "LureObject"@en ; 
    rdfs:comment " An object or set of objects used to attract an adversary that has the perception of high value regardless if it actually has high value."@en ; 
    rdfs:subClassOf uco-core:UcoObject ;
    sh:targetClass engage:LureObject . 
 

engage:Malware a owl:Class, 
        sh:NodeShape ; 
    rdfs:label "Malware"@en ; 
    rdfs:comment "Malware is an explicit, complex, multi-functional, crafted tool, software, or program for malicious purposes. Not all malicious tools are Malware though."@en ; 
    rdfs:subClassOf uco-tool:MaliciousTool ; 
    sh:targetClass engage:Malware . 

 

engage:Narrative a owl:Class, 
        sh:NodeShape ; 
    rdfs:label "Narrative"@en ; 
    rdfs:comment "A narrative is a script of all expected sequence of actions, events, entities and their interactions."@en ; 
    rdfs:subClassOf uco-core:UcoObject ; 
    sh:property [ sh:class uco-core:UcoObject ;
            sh:minCount 1 ;
            sh:nodeKind sh:BlankNodeOrIRI ;
            sh:path engage:hasStoryline ] ;
    sh:targetClass engage:Narrative . 

 

engage:PocketLitter a owl:Class, 
        sh:NodeShape ; 
    rdfs:label "PocketLitter"@en ; 
    rdfs:comment "Pocket litter describes objects placed prior or during an adversary engagement operation for the purpose of realism."@en ; 
    rdfs:subClassOf uco-core:UcoObject ; 
    sh:targetClass engage:PocketLitter . 

 

engage:Resource a owl:Class, 
        sh:NodeShape ; 
    rdfs:label "Resource"@en ; 
    rdfs:comment " A resource can be a tool, location or object which requires some operational cost to enable availability."@en ; 
    rdfs:subClassOf uco-core:UcoObject ; 
    sh:targetClass engage:Resource . 

 

engage:Sandbox a owl:Class, 
        sh:NodeShape ; 
    rdfs:label "Sandbox"@en ; 
    rdfs:comment " A controlled environment intended for malware detonation and malware analysis."@en ; 
    rdfs:subClassOf uco-core:UcoObject ; 
    sh:targetClass engage:Sandbox . 




engage:Stage a owl:Class,
        sh:NodeShape ;
    rdfs:label "Stage"@en ;
    rdfs:comment "A stage is a desired perception of an object or environment for an intended audience or entity which actors act/perform within and upon."@en ;
    rdfs:subClassOf uco-core:UcoObject ;
    sh:targetClass engage:Stage .

 

engage:Storyline a owl:Class, 
        sh:NodeShape ; 
    rdfs:label "Storyline"@en ; 
    rdfs:comment "A storyline is an indexed sequence of monotonic events as an expected trajectory for a narrative."@en ; 
    rdfs:subClassOf engage:Narrative ; 
    sh:targetClass engage:Storyline . 
 

engage:hasEventScript a owl:ObjectProperty, 
        sh:NodeShape ; 
    rdfs:label "hasEventScript"@en ; 
    rdfs:comment "An event script is relationship between the event object and the set of actions."@en ; 
    rdfs:range uco-core:UcoObject .
 

engage:hasStoryline a owl:ObjectProperty, 
        sh:NodeShape ; 
    rdfs:label "hasStoryline"@en ; 
    rdfs:comment "A storyline is exclusive to a narrative."@en ; 
    rdfs:range engage:Storyline .

engage:honeypotInteractionType a owl:DatatypeProperty ;
    rdfs:label "honeypotInteractionType"@en ;
    rdfs:comment "The interaction class intended for a honeypot."@en ;
    rdfs:range [ a rdfs:Datatype ;
            owl:unionOf ( vocabulary:HoneypotInteractionTypeVocab xsd:string ) ] .


identity:approachIdentifier a owl:DatatypeProperty ;
    rdfs:label "approachIdentifier"@en ;
    rdfs:comment "The unique identifier of the MITRE ENGAGE approach."@en ;
    rdfs:range xsd:string .

identity:goalIdentifier a owl:DatatypeProperty ;
    rdfs:label "goalIdentifier"@en ;
    rdfs:comment "The unique identifier of the MITRE ENGAGE goal."@en ;
    rdfs:range xsd:string .

 

engage:Persona a owl:Class, 
        sh:NodeShape ; 
    rdfs:label "Persona"@en ; 
    rdfs:comment " An persona is a facticious entity created to serve a purpose in a deception operation."@en ; 
    rdfs:subClassOf uco-identity:Identity ;
    sh:targetClass engage:Persona . 

identity:tacticIdentifier a owl:DatatypeProperty ;
    rdfs:label "tacticIdentifier"@en ;
    rdfs:comment "The unique identifier of the MITRE ATT&CK tactic."@en ;
    rdfs:range xsd:string .

identity:teamIdentifier a owl:DatatypeProperty ;
    rdfs:label "teamIdentifier"@en ;
    rdfs:comment "The unique identifier of a team."@en ;
    rdfs:range xsd:string .

identity:techniqueIdentifier a owl:DatatypeProperty ;
    rdfs:label "techniqueIdentifier"@en ;
    rdfs:comment "The unique identifier of the MITRE ATT&CK technique."@en ;
    rdfs:range xsd:string .

 

objective:Denial a owl:Class, 
        sh:NodeShape ; 
    rdfs:label "Denial"@en ; 
    rdfs:comment " An denial objective is to limit an adversary's capabilities or accessibility to a resource."@en ; 
    rdfs:subClassOf objective:Objective ;
    sh:targetClass objective:Denial . 
 

objective:ElicitBehavior a owl:Class, 
        sh:NodeShape ; 
    rdfs:label "ElicitBehavior"@en ; 
    rdfs:comment " An elicit behavior objective is to have an adversary or target object to exhibit some expected behavior."@en ; 
    rdfs:subClassOf objective:Objective ;
    sh:targetClass objective:ElicitBehavior . 
 

objective:Evasion a owl:Class, 
        sh:NodeShape ; 
    rdfs:label "Evasion"@en ; 
    rdfs:comment " An evasion objective is to avoid detection from some defense or entity."@en ; 
    rdfs:subClassOf objective:Objective ;
    sh:targetClass objective:Evasion . 
 

objective:Exfilitration a owl:Class, 
        sh:NodeShape ; 
    rdfs:label "Exfilitration"@en ; 
    rdfs:comment " An exfilitrate objective is an adversary objective to move native data to external sources."@en ; 
    rdfs:subClassOf objective:Objective ;
    sh:targetClass objective:Exfilitration . 
 

objective:hasObjective a owl:ObjectProperty, 
        sh:NodeShape ; 
    rdfs:label "hasObjective"@en ; 
    rdfs:comment "An object which can be associated with an objective."@en ; 
    rdfs:subClassOf uco-core:UcoObject ;	
    sh:targetClass objective:hasObjective . 
 

objective:Lure a owl:Class, 
        sh:NodeShape ; 
    rdfs:label "Lure"@en ; 
    rdfs:comment " An resource lure objective is have an adversary laterally move or take actions to reach some target lure, usually performed through the deployment of breadcrumbs and honeypots."@en ; 
    rdfs:subClassOf objective:Objective ;
    sh:targetClass objective:Lure . 


objective:Objective a owl:Class, 
        sh:NodeShape ; 
    rdfs:label "Objective"@en ; 
    rdfs:comment " An objective is associated with a sequence of actions which is reasoned and optimized for in the context of adversarial engagement."@en ; 
    rdfs:subClassOf uco-core:UcoObject ;	
    sh:property [ sh:datatype xsd:Literal ;
            sh:maxCount 1 ;
            sh:nodeKind sh:BlankNodeOrIRI ;
            sh:path identity:tacticIdentifier ] ,
	[ sh:datatype xsd:Literal ;
				sh:maxCount 1 ;
				sh:nodeKind sh:BlankNodeOrIRI ;
				sh:path identity:goalIdentifier ] ;
    sh:targetClass objective:Objective . 
 

objective:Persistence a owl:Class, 
        sh:NodeShape ; 
    rdfs:label "Persistence"@en ; 
    rdfs:comment " An persistence objective is maintain availability and access to some resource."@en ; 
    rdfs:subClassOf objective:Objective ;
    sh:targetClass objective:Persistence . 
 

objective:Reconnaissance a owl:Class, 
        sh:NodeShape ; 
    rdfs:label "Reconnaissance"@en ; 
    rdfs:comment " An reconnaissance objective is to gather information on a target entity or organization including by not limited to behavior, tactics, techniques, procedures and preferences."@en ; 
    rdfs:subClassOf objective:Objective ;
    sh:targetClass objective:Reconnaissance . 
 

objective:TimeSink a owl:Class, 
        sh:NodeShape ; 
    rdfs:label "TimeSink"@en ; 
    rdfs:comment " An time sink objective is to increase an adversary's operation time cost by having them interact with objects in a network."@en ; 
    rdfs:subClassOf objective:Objective ;
    sh:targetClass objective:TimeSink . 
 

objective:Track a owl:Class, 
        sh:NodeShape ; 
    rdfs:label "Track"@en ; 
    rdfs:comment " An track objective is to be capable of identifying and tracing an adversary throughout a network."@en ; 
    rdfs:subClassOf objective:Objective ;
    sh:targetClass objective:Track . 
 

objective:Trap a owl:Class, 
        sh:NodeShape ; 
    rdfs:label "Trap"@en ; 
    rdfs:comment " An trap objective is to limit an adversary's scope of reachability to a confined environment."@en ; 
    rdfs:subClassOf objective:Objective ,
		objective:Denial ;
    sh:targetClass objective:Trap . 



role:Team a owl:Class,
        sh:NodeShape ;
    rdfs:label "Team"@en ;
    rdfs:comment "The conventional reference to group of agents that are associated with some unified identity with a team objective"@en ;
    rdfs:subClassOf uco-identity:Organization ;
    sh:property [ sh:datatype xsd:Literal ;
            sh:maxCount 1 ;
            sh:nodeKind sh:BlankNodeOrIRI ;
            sh:path identity:teamIdentifier ] ;
    sh:targetClass role:Team .
	





vocabulary:HoneypotInteractionTypeVocab a rdfs:Datatype ;
    rdfs:label "Action Name Vocabulary"@en-US ;
    rdfs:comment "Defines a vocabulary of honeypot interaction characteristics."@en ;
    rdfs:subClassOf rdfs:Resource ;
    owl:oneOf ( "High"^^vocabulary:HoneypotTypeVocab "Low"^^vocabulary:HoneypotTypeVocab "Dynamic"^^vocabulary:HoneypotTypeVocab ) .

