
@prefix engage: <https://ontology.adversaryengagement.org/ae/engage/> . 
@prefix identity: <https://ontology.adversaryengagement.org/ae/identity/> .
@prefix objective: <https://ontology.RedTeamengagement.org/ae/objective/> . 
@prefix owl: <http://www.w3.org/2002/07/owl#> . 
@prefix rdfs: <http://www.w3.org/2000/01/rdf-schema#> . 
@prefix role: <https://ontology.adversaryengagement.org/ae/role/> .
@prefix sh: <http://www.w3.org/ns/shacl#> . 
@prefix uco-core: <https://ontology.unifiedcyberontology.org/uco/core/> . 
@prefix uco-identity: <https://ontology.unifiedcyberontology.org/uco/identity/> . 
@prefix uco-role: <https://ontology.unifiedcyberontology.org/uco/role/> .


 
	
identity:BlueTeam a identity:Team ;
  rdfs:label "BlueTeam"@en;
  rdfs:comment "An BlueTeam is an instance of a team with defender objectives."@en;
  rdfs:range	uco-identity:Organization .


 

identity:Persona a owl:Class, 
        sh:NodeShape ; 
    rdfs:label "Persona"@en ; 
    rdfs:comment " An persona is a facticious entity created to serve a purpose in a deception operation."@en ; 
    rdfs:subClassOf uco-identity:Identity ;
    sh:targetClass identity:Persona . 

 
	
identity:PurpleTeam a identity:Team ;
  rdfs:label "PurpleTeam"@en;
  rdfs:comment "An PurpleTeam is an instance of a team with post analysis objectives."@en;
  rdfs:range	uco-identity:Organization .


 
	
identity:RedTeam a identity:Team ;
  rdfs:label "RedTeam"@en;
  rdfs:comment "An RedTeam is an instance of a team with adversary objectives."@en;
  rdfs:range	uco-identity:Organization .



identity:Team a owl:Class,
        sh:NodeShape ;
    rdfs:label "Team"@en ;
    rdfs:comment "The conventional reference to group of identities that are associated with some unified identity with a team objective"@en ;
    rdfs:subClassOf uco-identity:Organization ;
    sh:property [ sh:class engage:Objective ;
            sh:nodeKind sh:IRI ;
            sh:path objective:hasObjective ] ;
    sh:targetClass identity:Team .
	
