
@prefix attack: <https://ontology.adversaryengagement.org/ae/attack/> .
@prefix owl: <http://www.w3.org/2002/07/owl#> .
@prefix rdf: <http://www.w3.org/1999/02/22-rdf-syntax-ns#> .
@prefix rdfs: <http://www.w3.org/2000/01/rdf-schema#> .
@prefix sh: <http://www.w3.org/ns/shacl#> .
@prefix uco-action: <https://ontology.unifiedcyberontology.org/uco/action/> .
@prefix uco-core: <https://ontology.unifiedcyberontology.org/uco/core/> . 
@prefix uco-observable: <https://ontology.unifiedcyberontology.org/uco/observable/> .
@prefix vocabulary: <https://ontology.adversaryengagement.org/ae/vocabulary/> .
@prefix xsd: <http://www.w3.org/2001/XMLSchema#> .




attack:Attack a owl:Class,
        sh:NodeShape ;
    rdfs:label "Attack"@en ;
    rdfs:comment "An attack is some adversarial behavioral classification from an attack framework."@en ;
    rdfs:subClassOf uco-action:ActionPattern ;
    sh:targetClass attack:Attack .



attack:cyberKillChain a owl:Class,
        sh:NodeShape ;
    rdfs:label "cyberKillChain"@en ;
    rdfs:comment "An cyber kill chain is a ordered sequence of actions or events describing a lifecycle from some framework."@en ;
    rdfs:subClassOf uco-action:ActionLifecycle ;
    sh:targetClass attack:cyberKillChain .



attack:cyberKillChainFacet a owl:Class,
        sh:NodeShape ;
    rdfs:label "cyberKillChainFacet"@en ;
    rdfs:comment "An cyber kill chain is a ordered sequence of actions describing a lifecycle from an attack framework."@en ;
    rdfs:subClassOf uco-core:Facet ;
    sh:targetClass attack:cyberKillChainFacet .


attack:LockheedMartinCyberKillChainFacet a owl:Class,
        sh:NodeShape ;
    rdfs:label "LockheedMartinCyberKillChainFacet"@en ;
    rdfs:comment "A concept that references Lockheed Martin's cyber kill chain."@en ;
    rdfs:subClassOf attack:cyberKillChainFacet ;
    sh:targetClass attack:LockheedMartinCyberKillChainFacet .



attack:MitreCyberKillChainFacet a owl:Class,
        sh:NodeShape ;
    rdfs:label "MitreCyberKillChainFacet"@en ;
    rdfs:comment "An cyber kill chain is a ordered sequence of actions describing a lifecycle from the MITRE ATT&CK framework."@en ;
    rdfs:subClassOf attack:cyberKillChainFacet ;
    sh:targetClass attack:MitreCyberKillChainFacet .



attack:MitreFacet a owl:Class,
        sh:NodeShape ;
    rdfs:label "MitreFacet"@en ;
    rdfs:comment "A concept that references MITRE ATT&CK'S framework."@en ;
    rdfs:subClassOf uco-core:Facet ;
    sh:targetClass attack:MitreFacet .



attack:MitreProcedureFacet a owl:Class,
        sh:NodeShape ;
    rdfs:label "MitreProcedureFacet"@en ;
    rdfs:comment "An attack procedure from MITRE ATT&CK framework."@en ;
    rdfs:subClassOf attack:MitreTechniqueFacet ;
    sh:targetClass attack:MitreProcedureFacet .



attack:MitreTacticFacet a owl:Class,
        sh:NodeShape ;
    rdfs:label "MitreTacticFacet"@en ;
    rdfs:comment "An attack tactic from MITRE ATT&CK framework."@en ;
    rdfs:subClassOf attack:MitreFacet ;
    sh:targetClass attack:MitreTacticFacet .



attack:MitreTechinqueType a owl:DatatypeProperty ;
    rdfs:label "MitreTechinqueType"@en ;
    rdfs:comment "Mitre ATT&CK's techniques."@en ;
    rdfs:range [ a rdfs:Datatype ;
            owl:unionOf ( vocabulary:MitreTechinqueTypeVocab xsd:string ) ] .


attack:MitreTechniqueFacet a owl:Class,
        sh:NodeShape ;
    rdfs:label "MitreTechniqueFacet"@en ;
    rdfs:comment "An attack technique from MITRE ATT&CK framework."@en ;
    rdfs:subClassOf attack:MitreTacticFacet ;
    sh:targetClass attack:MitreTechniqueFacet .