
@prefix engage: <https://ontology.adversaryengagement.org/ae/engage/> .
@prefix identity: <https://ontology.adversaryengagement.org/ae/identity/> .
@prefix owl: <http://www.w3.org/2002/07/owl#> .
@prefix rdf: <http://www.w3.org/1999/02/22-rdf-syntax-ns#> .
@prefix rdfs: <http://www.w3.org/2000/01/rdf-schema#> .
@prefix role: <https://ontology.adversaryengagement.org/ae/role/> .
@prefix sh: <http://www.w3.org/ns/shacl#> .
@prefix uco-core: <https://ontology.unifiedcyberontology.org/uco/core/> .
@prefix uco-identity: <https://ontology.unifiedcyberontology.org/uco/identity/> .
@prefix uco-observable: <https://ontology.unifiedcyberontology.org/uco/observable/> .
@prefix uco-role: <https://ontology.unifiedcyberontology.org/uco/role/> .
@prefix vocabulary: <https://ontology.adversaryengagement.org/ae/vocabulary/> .
@prefix xsd: <http://www.w3.org/2001/XMLSchema#> . 



role:adversary a owl:Class,
        sh:NodeShape ;
    rdfs:label "adversary"@en ;
    rdfs:comment "An adversary is a contextual reference to an entity that has some opposing objective to a network's confidentiality, integrity, availability or any security objective."@en ;
    rdfs:subClassOf uco-identity:Person ,
		uco-role:Role ;
    sh:targetClass role:adversary .


role:defender a owl:Class,
        sh:NodeShape ;
    rdfs:label "defender"@en ;
    rdfs:comment "An defender is a contextual reference to an entity whose objective is aligned with a network's confidentiality, integrity, availability or security objective."@en ;
    rdfs:subClassOf uco-identity:Person ,
		uco-role:Role ;
    sh:targetClass role:defender .


role:hasHumanTeamMember a owl:ObjectProperty ;
    rdfs:label "hasHumanTeamMember"@en ;
    rdfs:comment "A human team member is a grouping of identifying characteristics unique to an human entity as an individual."@en ;
    rdfs:range role:humanTeamMember .


role:hasTargetEntity a owl:ObjectProperty ;
    rdfs:label "hasTargetEntity"@en ;
    rdfs:comment "A targetIdentity is an entity or team which a defender, adversary or team performs action to or interact with."@en ;
    rdfs:range role:TargetEntity .
	



role:hasTeam a owl:ObjectProperty ;
    rdfs:label "hasTeam"@en ;
    rdfs:comment "The conventional reference to group of agents that are associated with some unified identity with a team objective"@en ;
    rdfs:range role:Team .
	



role:humanTeamMember a owl:Class,
        sh:NodeShape ;
    rdfs:label "humanTeamMember"@en ;
    rdfs:comment "A human team member is a grouping of identifying characteristics unique to an human entity as an individual."@en ;
    rdfs:subClassOf uco-identity:Identity ,
		uco-role:Role ;
    sh:targetClass role:humanTeamMember .


role:TargetEntity a owl:Class,
        sh:NodeShape ;
    rdfs:label "Target"@en ;
    rdfs:comment "A targetIdentity is an entity or team which a defender, adversary or team performs action to or interact with."@en ;
    rdfs:subClassOf uco-identity:Identity;
    sh:targetClass role:TargetEntity .
	



role:Team a owl:Class,
        sh:NodeShape ;
    rdfs:label "Team"@en ;
    rdfs:comment "The conventional reference to group of agents that are associated with some unified identity with a team objective"@en ;
    rdfs:subClassOf uco-identity:Organization ;
    sh:targetClass role:Team .
	


identity:TeamFacet a owl:Class,
        sh:NodeShape ;
    rdfs:label "TeamFacet"@en ;
    rdfs:comment "Team is a grouping of entities for describing cooperative relationships among its entity members."@en ;
    rdfs:subClassOf uco-identity:IdentityFacet ;
	
    sh:property [ sh:datatype xsd:string ;
            sh:maxCount 1 ;
            sh:nodeKind sh:Literal ;
            sh:path identity:teamName ],
        [ sh:class uco-core:UcoObject ;
            sh:nodeKind sh:Literal ;
            sh:path identity:hasHumanTeamMember ],
		[ sh:datatype xsd:string ;
					sh:maxCount 1 ;
					sh:minCount 1 ;
					sh:nodeKind sh:Literal ;
					sh:path identity:teamIdentifier ],
        [ sh:datatype vocabulary:TeamTypeVocab ;
            sh:message "Value is outside the default vocabulary TeamTypeVocab." ;
            sh:path role:teamType ;
            sh:severity sh:Info ],
        [ sh:maxCount 1 ;
            sh:nodeKind sh:Literal ;
            sh:or ( [ sh:datatype vocabulary:TeamTypeVocab ] [ sh:datatype xsd:string ] ) ;
            sh:path role:teamType ],
        [ sh:message "Value is not member of the vocabulary TeamTypeVocab." ;
            sh:or ( [ sh:datatype vocabulary:TeamTypeVocab ;
                        sh:in vocabulary:TeamTypeVocab-members ] [ sh:datatype xsd:string ] ) ;
            sh:path role:teamType ] ;
		
    sh:targetClass role:TeamFacet .


identity:teamMember a owl:Class,
        sh:NodeShape ;
    rdfs:label "teamMember"@en ;
    rdfs:comment "A team member is an entity or group of entities assigned to an identifiable team."@en ;
    rdfs:subClassOf uco-identity:Identity,
		uco-role:Role ;
    sh:targetClass identity:teamMember .

role:teamType a owl:DatatypeProperty ;
    rdfs:label "teamType"@en ;
    rdfs:comment "The traditional color-typing for a team."@en ;
    rdfs:range [ a rdfs:Datatype ;
            owl:unionOf ( vocabulary:TeamTypeVocab xsd:string ) ] .